Rework effects

theories/Morphisms.v
@@ -1,22 +1,45 @@
-(* Effects form a category where the arrows are effect morphisms.
- *
- * These morphisms can be used to transport itrees from one effect
- * to another.
- *
- * Some morphisms interpret effects using additional structure.
- * In general, this additional structure is monadic in nature.
+(** The semantics of an interaction tree [itree E ~> M] can be
+    derived from semantics given for every individual effect
+    [E ~> M].
+
+    We define the following terminology for this library.
+    Other sources may have different usages for the same or related
+    words.
+
+    The notation [E ~> F] means [forall T, E T -> F T]
+    (in [ITree.Basics]).
+    It can mean many things, including the following.
+
+    - The semantics of itrees are given as monad morphisms
+      [itree E ~> M], also called "interpreters".
+
+    - "Itree interpreters" (or "itree morphisms") are monad morphisms
+      [itree E ~> itree F]. Most interpreters in this library are
+      actually itree interpreters.
+
+    This module provides various ways of defining interpreters
+    from effect handlers and other similar structures.
+
+    - "Effect handlers" are functions [E ~> M] where [M] is a monad.
+
+    - "Itree effect handlers" are functions [E ~> itree F].
+
+    Categorically, this boils down to saying that [itree] is a free
+    monad (not quite, but close enough).
  *)
 
-From ExtLib.Structures Require Import
-     Functor.
+From ExtLib Require
+     Structures.Monoid.
 
 From ITree Require Import
-     Core OpenSum.
+     Basics
+     Core
+     Effect.Sum.
 
 Open Scope itree_scope.
 
-(* [itreeF] eliminator, where the codomain is in the [itree]
-   monad, a building block for itree monad morphisms. *)
+(** [itreeF] eliminator, where the codomain is in the [itree]
+    monad, a building block for itree monad morphisms. *)
 Definition handleF {E F : Type -> Type} {I R : Type}
            (tau : I -> itree F R)
            (vis : forall U, E U -> (U -> I) -> itree F R)
@@ -28,147 +51,150 @@ Definition handleF {E F : Type -> Type} {I R : Type}
   end.
 Hint Unfold handleF.
 
-(* Shallow effect handling: pass the first [Vis] node to the
-   given handler [h]. *)
+(** Shallow effect handling: pass the first [Vis] node to the
+    given handler [h]. *)
 Definition handle {E F : Type -> Type} {R : Type}
            (h : forall U, E U -> (U -> itree E R) -> itree F R) :
   itree E R -> itree F R :=
   cofix handle_ t := handleF handle_ h (observe t).
 Hint Unfold handle.
 
-(* * Homomorphisms between effects *)
-Definition eff_hom (E E' : Type -> Type) : Type :=
-  forall t, E t -> itree E' t.
-
-(* An [eff_hom] can be used to transport itrees between different
-   effects. *)
-Definition interp {E F : Type -> Type} {R : Type}
-           (f : eff_hom E F)
-: itree E R -> itree F R :=
+(** An itree effect handler [E ~> itree F] defines an
+    itree morphism [itree E ~> itree F]. *)
+Definition interp {E F : Type -> Type} (h : E ~> itree F) :
+  itree E ~> itree F := fun R =>
   cofix interp_ t :=
     handleF interp_
-            (fun _ e k => Tau (ITree.bind (f _ e)
+            (fun _ e k => Tau (ITree.bind (h _ e)
                                           (fun x => interp_ (k x))))
             (observe t).
 (* N.B.: the guardedness of this definition relies on implementation
    details of [bind]. *)
 
-(* Interpret the first effect [E] in a sum [E +' F] into
-   the rest of the sum [F].
+(** Interpret the first effect [E] in a sum [E +' F] into
+    the rest of the sum [F].
 
-   Compared to [interp], this inserts fewer [Tau] nodes, which
-   allows a few equations to be bisimularities ([eq_itree]) instead
-   of up-to-tau equivalences ([eutt]).
+    Compared to [interp], this inserts fewer [Tau] nodes, which
+    allows a few equations to be bisimularities ([eq_itree]) instead
+    of up-to-tau equivalences ([eutt]).
  *)
-Definition interp1 {E F : Type -> Type} {R : Type}
-           (f : eff_hom E F) :
-  itree (E +' F) R -> itree F R :=
+Definition interp1 {E F : Type -> Type} (h : E ~> itree F) :
+  itree (E +' F) ~> itree F := fun R =>
   cofix interp1_ t :=
     handleF interp1_
             (fun _ ef k =>
                match ef with
-               | inlE e => Tau (ITree.bind (f _ e)
+               | inl1 e => Tau (ITree.bind (h _ e)
                                            (fun x => interp1_ (k x)))
-               | inrE f => Vis f (fun x => interp1_ (k x))
+               | inr1 f => Vis f (fun x => interp1_ (k x))
                end)
             (observe t).
 
-(* * Effects form a category
- * The objects are effects: i.e. `Type -> Type`
- * The morphisms from `a` to `b` are `eff_hom a b`
- *)
+(** A plain effect morphism [E ~> F] defines an itree morphism
+    [itree E ~> itree F]. *)
+Definition translate {E F : Type -> Type} (h : E ~> F) :
+  itree E ~> itree F := fun R =>
+  cofix translate_ t :=
+    handleF translate_
+            (fun _ e k => Vis (h _ e) (fun x => translate_ (k x)))
+            (observe t).
+
+(** Effects [E, F : Type -> Type] and itree [E ~> itree F] form a
+    category. *)
+(* TODO: check that [itree] is a monad, so that category is its
+   Kleisli category. *)
 
 (* todo(gmm): it would be good to have notation for this.
  * - if there was a "category" class like in Haskell, then we could
  *   get composition from something like that.
  *)
-Definition eh_compose {A B C} (g : eff_hom B C) (f : eff_hom A B)
-: eff_hom A C :=
-  fun _ e =>
-    interp g (f _ e).
+Definition eh_compose {A B C} (g : B ~> itree C) (f : A ~> itree B) :
+  A ~> itree C :=
+  fun _ e => interp g _ (f _ e).
 
-Definition eh_id {A} : eff_hom A A := @ITree.liftE A.
+Definition eh_id {A} : A ~> itree A := @ITree.liftE A.
 
-Section eff_hom_state.
-  Variable s : Type.
-  Variable E E' : Type -> Type.
+(** Standard interpreters *)
 
-  (* * Stateful homomorphisms between effects *)
-  Definition eff_hom_s : Type :=
-    forall t, E t -> s -> itree E' (s * t).
+Import ITree.Basics.Monads.
 
-  (* question(gmm): Should we export this using `stateT`? That is,
-   *
-   * interp_state {E F S} (f : eff_hom_s S E F) (R : Type)
-   *   itree E R -> stateT S (itree F) R.
-   *
-   * a nice benefit of this is that it makes the structure a bit more
-   * explicit (and hints at the generalization to arbitary monads).
-   *)
-  Variable f : eff_hom_s.
-  CoFixpoint interp_state (R : Type) (t : itree E R) (st : s)
-  : itree E' (s * R) :=
-    match t.(observe) with
-    | RetF r => Ret (st, r)
-    | VisF e k => ITree.bind (f _ e st) (fun '(s',x) => Tau (interp_state _ (k x) s'))
-    | TauF t => Tau (interp_state _ t st)
-    end.
-End eff_hom_state.
-Arguments interp_state {_ _ _} _ [_] _ _.
+(* TODO: refactor these three... *)
 
-(* * Reader homomorphisms between effects *)
-Section eff_hom_reader.
-  Variable s : Type.
-  Variable E E' : Type -> Type.
+(* Stateful handlers [E ~> stateT S (itree F)] and morphisms
+   [E ~> state S] define stateful itree morphisms
+   [itree E ~> stateT S (itree F)]. *)
 
-  Definition eff_hom_r : Type :=
-    forall t, E t -> s -> itree E' t.
+Definition interp_state {E F S} (h : E ~> stateT S (itree F)) :
+  itree E ~> stateT S (itree F) :=
+  fun R =>
+    cofix interp_state_ t s :=
+      match t.(observe) with
+      | RetF r => Ret (s, r)
+      | VisF e k =>
+        Tau (ITree.bind (h _ e s) (fun sx =>
+               interp_state_ (k (snd sx)) (fst sx)))
+      | TauF t => Tau (interp_state_ t s)
+      end.
 
-  Variable f : eff_hom_r.
-  CoFixpoint interp_reader (R : Type) (t : itree E R) (st : s) : itree E' R :=
-    match t.(observe) with
-    | RetF r => Ret r
-    | VisF e k => ITree.bind (f _ e st) (fun x => Tau (interp_reader _ (k x) st))
-    | TauF t => Tau (interp_reader _ t st)
-    end.
+Definition interp1_state {E F S} (h : E ~> stateT S (itree F)) :
+  itree (E +' F) ~> stateT S (itree F) :=
+  fun R =>
+    cofix interp1_state_ t s :=
+      match t.(observe) with
+      | RetF r => Ret (s, r)
+      | VisF ef k =>
+        match ef with
+        | inl1 e =>
+          let sx := h _ e s in
+          Tau (ITree.bind (h _ e s) (fun sx =>
+                 interp1_state_ (k (snd sx)) (fst sx)))
+        | inr1 f => Vis f (fun x => interp1_state_ (k x) s)
+        end
+      | TauF t => Tau (interp1_state_ t s)
+      end.
 
-End eff_hom_reader.
+Definition translate1_state {E F S} (h : E ~> state S) :
+  itree (E +' F) ~> stateT S (itree F) :=
+  fun R =>
+    cofix translate1_state_ t s :=
+      match t.(observe) with
+      | RetF r => Ret (s, r)
+      | VisF ef k =>
+        match ef with
+        | inl1 e => let sx := h _ e s in
+                    Tau (translate1_state_ (k (snd sx)) (fst sx))
+        | inr1 f => Vis f (fun x => translate1_state_ (k x) s)
+        end
+      | TauF t => Tau (translate1_state_ t s)
+      end.
 
-Arguments interp_reader {_ _ _} _ [_] _ _.
+(** The "reader" and "writer" variants are specializations
+    of the above stateful morphisms when the state cannot
+    be changed or read (i.e., append only). *)
 
-Require Import ExtLib.Structures.Monoid.
+Definition interp_reader {E F R} (h : R -> E ~> itree F) :
+  R -> itree E ~> itree F :=
+  fun r => interp (h r).
 
-(* * Writer homomorphisms between effects *)
-Section eff_hom_writer.
-  Variable s : Type.
-  Variable E E' : Type -> Type.
+Definition interp1_reader {E F R} (h : R -> E ~> itree F) :
+  R -> itree (E +' F) ~> itree F :=
+  fun r => interp1 (h r).
 
-  Definition eff_hom_w : Type :=
-    forall t, E t -> itree E' (s * t).
+Definition translate1_reader {E F R} (h : R -> E ~> identity) :
+  R -> itree (E +' F) ~> itree F :=
+  fun r => interp1 (fun _ e => Ret (h r _ e)).
 
-  Context {Monoid_s : Monoid s}.
-  Variable f : eff_hom_w.
+Import ExtLib.Structures.Monoid.
 
-  (* Note that we have to give an intepretation in terms of state in order
-   * to pass the productivity checker. This definition is equivalent to:
-   *
-   * CoFixpoint interp_reader (R : Type) (t : itree E R) (st : s) : itree E' R :=
-   *   match t with
-   *   | Ret r => Ret r
-   *   | Vis e k => Core.bindTau (f _ e st)
-   *     (fun x => fmap (fun '(s',x) => (monoid_plus Monoid_s s s', x))
-   *                    (interp_writer _ (k x) st))
-   *   | Tau t => Tau (interp_writer _ t st)
-   *   end.
-   *)
-  Definition interp_writer (R : Type) (t : itree E R) : itree E' (s * R) :=
+Definition map_fst {A A' B} (f : A -> A') : A * B -> A' * B :=
+  fun '(a, b) => (f a, b).
+
+Definition interp_writer {E F W} {Monoid_W : Monoid W} (h : E ~> writerT W (itree F)) :
+  itree E ~> writerT W (itree F) :=
+  fun _ t =>
     interp_state
-      (fun _ e s => fmap (fun '(s',x) => (monoid_plus Monoid_s s s', x)) (f _ e))
-      t (monoid_unit Monoid_s).
-
-End eff_hom_writer.
-
-Arguments interp_writer {_ _ _ _} _ [_] _.
+      (fun _ e s => ITree.map (map_fst (monoid_plus Monoid_W s)) (h _ e))
+      _ t (monoid_unit Monoid_W).
 
 (* todo(gmm): this can be stronger if we allow for a `can_returnE` *)
 Inductive can_return {E : Type -> Type} {t : Type} : itree E t -> t -> Prop :=
@@ -177,8 +203,8 @@ Inductive can_return {E : Type -> Type} {t : Type} : itree E t -> t -> Prop :=
 | can_return_Vis {u e k} {x: u} {res} (_ : can_return (k x) res)
   : can_return (Vis e k) res.
 
-(* A propositional "interpreter"
- * This can be useful for non-determinism.
+(** A propositional "interpreter"
+    This can be useful for non-determinism.
  *)
 Section interp_prop.
   Context {E F : Type -> Type}.
@@ -202,8 +228,7 @@ Section interp_prop.
 End interp_prop.
 Arguments eff_hom_prop _ _ : clear implicits.
 
-(* * An extensional effect morphism
- *)
+(** An extensional stateful handler *)
 Section eff_hom_e.
   Context {E F : Type -> Type}.
 
@@ -216,48 +241,50 @@ Section eff_hom_e.
    * but you have the usual conditions on strictly positive uses
    *)
   CoInductive eff_hom_e : Type :=
-  { eval : forall t, E t -> itree F (t * eff_hom_e) }.
+  { eval : forall t, E t -> itree F (eff_hom_e * t) }.
 
-  CoFixpoint interp_e (f : eff_hom_e) {t} (tr : itree E t)
-  : itree F t :=
-    match tr.(observe) with
-    | RetF v => Ret v
-    | VisF e k =>
-      ITree.bind (f.(eval) _ e) (fun '(x, f') => Tau (interp_e f' (k x)))
-    | TauF tr => Tau (interp_e f tr)
-    end.
+  CoFixpoint interp_e (h : eff_hom_e) : itree E ~> itree F :=
+    fun R t =>
+      handleF (interp_e h _)
+              (fun _ e k => ITree.bind (h.(eval) _ e)
+                     (fun '(h', x) => Tau (interp_e h' _ (k x))))
+              (observe t).
+
 End eff_hom_e.
 
 Section into.
   Context {E F : Type -> Type}.
 
-  Definition into (h : eff_hom E F) : eff_hom (E +' F) F :=
+  Definition into (h : E ~> itree F) : (E +' F) ~> itree F :=
     fun _ e =>
       match e with
-      | inlE e => h _ e
-      | inrE e => ITree.liftE e
+      | inl1 e => h _ e
+      | inr1 e => ITree.liftE e
       end.
 
-  Definition into_state {s} (h : eff_hom_s s E F) : eff_hom_s s (E +' F) F :=
+  Definition into_state {s} (h : E ~> stateT s (itree F)) :
+    (E +' F) ~> stateT s (itree F) :=
     fun _ e s =>
       match e with
-      | inlE e => h _ e s
-      | inrE e => Vis e (fun x => Ret (s, x))
+      | inl1 e => h _ e s
+      | inr1 e => Vis e (fun x => Ret (s, x))
       end.
 
-  Definition into_reader {s} (h : eff_hom_r s E F) : eff_hom_r s (E +' F) F :=
-    fun _ e s =>
+  Definition into_reader {R} (h : R -> E ~> itree F) :
+    R -> E +' F ~> itree F :=
+    fun r _ e =>
       match e with
-      | inlE e => h _ e s
-      | inrE e => ITree.liftE e
+      | inl1 e => h r _ e
+      | inr1 e => ITree.liftE e
       end.
 
-  Definition into_writer {s} `{Monoid_s : Monoid s} (h : eff_hom_w s E F)
-  : eff_hom_w s (E +' F) F :=
+  Definition into_writer {W} (Monoid_W : Monoid W)
+             (h : E ~> writerT W (itree F))
+    : E +' F ~> writerT W (itree F) :=
     fun _ e =>
       match e with
-      | inlE e => h _ e
-      | inrE e => Vis e (fun x => Ret (monoid_unit Monoid_s, x))
+      | inl1 e => h _ e
+      | inr1 e => Vis e (fun x => Ret (monoid_unit Monoid_W, x))
       end.
 
   (* todo(gmm): is the a corresponding definition for `eff_hom_p`? *)
